\documentclass[../revisedmain.tex]{subfiles}
\begin{document}
	The reader should be familiar with $\displaystyle\frac{dy}{dx}$ at this point. Remember that what that means is the instantaneous change in $y$ with respect to the instantaneous change in $x$. This can be rewritten and solved for $dy$ as a function of $dx$. It's just as simple as getting $\displaystyle\frac{dy}{dx}$ on one side and multiplying by $dx$ so the equation looks like: $$\frac{dy}{dx}=f'(x)$$$$dy=f'(x)dx$$ Given the equation $x^2+y^2=1$, the differential equation will be: $$2x\frac{dx}{dx}+2y\frac{dy}{dx} = 0$$$$2y\frac{dy}{dx}=-2x$$$$dy=-\frac{x}{y}dx$$
\end{document}