\documentclass[../revisedmain.tex]{subfiles}
\begin{document}
	\paragraph{Example 1:} Find $\lim\limits_{x\to\infty}\frac{x^3-x+1}{4x^3+2x^2+x-1}$. A method for solving this particular type of problem is shown before Calculus, but here is the reason why it works:
	\begin{gather*}
		\lim_{x\to\infty}\frac{x^3-x+1}{4x^3+2x^2+x-1}=\frac{\infty}{\infty}
	\end{gather*}This is an indeterminate form so we can apply L'h\^opital's rule:
	\begin{gather*}
		\lim_{x\to\infty}\frac{x^3-x+1}{4x^3+2x^2+x-1}=\frac{\infty}{\infty}\\\\\\\\
		\lim_{x\to\infty}\frac{x^3-x+1}{4x^3+2x^2+x-1}=\lim_{x\to\infty}\frac{3x^2-1}{12x^2+4x+1}\\\\
		\lim_{x\to\infty}\frac{3x^2-1}{12x^2+4x+1}=\frac{\infty}{\infty}\\\\\\\\
		\lim_{x\to\infty}\frac{3x^2-1}{12x^2+4x+1}=\lim_{x\to\infty}\frac{6x}{24x+4}\\\\
		\lim_{x\to\infty}\frac{6x}{24x+4}=\lim_{x\to\infty}\frac{\infty}{\infty}\\\\\\\\
		\lim_{x\to\infty}\frac{6x}{24x+4}=\frac{6}{24}\\\\
		\lim_{x\to\infty}\frac{6}{24}=\frac{6}{24}=\frac{1}{4}\\
	\end{gather*}
\end{document}
